backend/RTLgenproof.v
@@ -366,17 +366,12 @@ Proof.
   intros. apply match_transform_partial_program; auto.
 Qed.
 
-Definition match_pol := match_pol (fun f tf => transl_fundef f = OK tf).
 
 Section CORRECTNESS.
 
 Variable prog: CminorSel.program.
 Variable tprog: RTL.program.
 Hypothesis TRANSL: match_prog prog tprog.
-
-Variable pol: CminorSel.policy.
-Variable tpol: RTL.policy.
-Hypothesis TRANSPOL: match_pol pol tpol.
 
 Let ge : CminorSel.genv := Genv.globalenv prog.
 Let tge : RTL.genv := Genv.globalenv tprog.
@@ -430,7 +425,7 @@ Lemma tr_move_correct:
   forall r1 ns r2 nd cs f sp rs m,
   tr_move f.(fn_code) ns r1 nd r2 ->
   exists rs',
-  star (step tpol) tge (State cs f sp ns rs m) E0 (State cs f sp nd rs' m) /\
+  star step tge (State cs f sp ns rs m) E0 (State cs f sp nd rs' m) /\
   rs'#r2 = rs#r1 /\
   (forall r, r <> r2 -> rs'#r = rs#r).
 Proof.
@@ -490,7 +485,7 @@ Definition transl_expr_prop
     (ME: match_env map e le rs)
     (EXT: Mem.extends m tm),
   exists rs', exists tm',
-     star (step tpol) tge (State cs f sp ns rs tm) E0 (State cs f sp nd rs' tm')
+     star step tge (State cs f sp ns rs tm) E0 (State cs f sp nd rs' tm')
   /\ match_env map (set_optvar dst v e) le rs'
   /\ Val.lessdef v rs'#rd
   /\ (forall r, In r pr -> rs'#r = rs#r)
@@ -505,7 +500,7 @@ Definition transl_exprlist_prop
     (ME: match_env map e le rs)
     (EXT: Mem.extends m tm),
   exists rs', exists tm',
-     star (step tpol) tge (State cs f sp ns rs tm) E0 (State cs f sp nd rs' tm')
+     star step tge (State cs f sp ns rs tm) E0 (State cs f sp nd rs' tm')
   /\ match_env map e le rs'
   /\ Val.lessdef_list vl rs'##rl
   /\ (forall r, In r pr -> rs'#r = rs#r)
@@ -520,7 +515,7 @@ Definition transl_condexpr_prop
     (ME: match_env map e le rs)
     (EXT: Mem.extends m tm),
   exists rs', exists tm',
-     plus (step tpol) tge (State cs f sp ns rs tm) E0 (State cs f sp (if v then ntrue else nfalse) rs' tm')
+     plus step tge (State cs f sp ns rs tm) E0 (State cs f sp (if v then ntrue else nfalse) rs' tm')
   /\ match_env map e le rs'
   /\ (forall r, In r pr -> rs'#r = rs#r)
   /\ Mem.extends m tm'.
@@ -563,7 +558,7 @@ Qed.
 Lemma transl_expr_Eop_correct:
   forall (le : letenv) (op : operation) (args : exprlist)
          (vargs : list val) (v : val),
-  eval_exprlist pol ge sp e cp m le args vargs ->
+  eval_exprlist ge sp e cp m le args vargs ->
   transl_exprlist_prop le args vargs ->
   eval_operation ge sp op vargs m = Some v ->
   transl_expr_prop le (Eop op args) v.
@@ -591,7 +586,7 @@ Qed.
 Lemma transl_expr_Eload_correct:
   forall (le : letenv) (chunk : memory_chunk) (addr : Op.addressing)
          (args : exprlist) (vargs : list val) (vaddr v : val),
-  eval_exprlist pol ge sp e cp m le args vargs ->
+  eval_exprlist ge sp e cp m le args vargs ->
   transl_exprlist_prop le args vargs ->
   Op.eval_addressing ge sp addr vargs = Some vaddr ->
   Mem.loadv chunk m vaddr = Some v ->
@@ -620,9 +615,9 @@ Qed.
 Lemma transl_expr_Econdition_correct:
   forall (le : letenv) (a: condexpr) (ifso ifnot : expr)
          (va : bool) (v : val),
-  eval_condexpr pol ge sp e cp m le a va ->
+  eval_condexpr ge sp e cp m le a va ->
   transl_condexpr_prop le a va ->
-  eval_expr pol ge sp e cp m le (if va then ifso else ifnot) v ->
+  eval_expr ge sp e cp m le (if va then ifso else ifnot) v ->
   transl_expr_prop le (if va then ifso else ifnot) v ->
   transl_expr_prop le (Econdition a ifso ifnot) v.
 Proof.
@@ -646,9 +641,9 @@ Qed.
 
 Lemma transl_expr_Elet_correct:
   forall (le : letenv) (a1 a2 : expr) (v1 v2 : val),
-  eval_expr pol ge sp e cp m le a1 v1 ->
+  eval_expr ge sp e cp m le a1 v1 ->
   transl_expr_prop le a1 v1 ->
-  eval_expr pol ge sp e cp m (v1 :: le) a2 v2 ->
+  eval_expr ge sp e cp m (v1 :: le) a2 v2 ->
   transl_expr_prop (v1 :: le) a2 v2 ->
   transl_expr_prop le (Elet a1 a2) v2.
 Proof.
@@ -714,10 +709,9 @@ Qed.
 
 Lemma transl_expr_Ebuiltin_correct:
   forall le ef al vl v,
-  eval_exprlist pol ge sp e cp m le al vl ->
+  eval_exprlist ge sp e cp m le al vl ->
   transl_exprlist_prop le al vl ->
   external_call ef ge cp vl m E0 v m ->
-  forall ALLOWED: Policy.allowed_call pol cp (External ef),
   transl_expr_prop le (Ebuiltin ef al) v.
 Proof.
   intros; red; intros. inv TE.
@@ -730,7 +724,6 @@ Proof.
   change (rs1#rd <- v') with (regmap_setres (BR rd) v' rs1).
   eapply exec_Ibuiltin; eauto.
   eapply eval_builtin_args_trivial.
-  eapply TRANSPOL; eauto. simpl; reflexivity.
   eapply external_call_symbols_preserved; eauto. apply senv_preserved.
   eauto.
 (* Match-env *)
@@ -748,10 +741,9 @@ Lemma transl_expr_Eexternal_correct:
   Genv.find_symbol ge id = Some b ->
   Genv.find_funct_ptr ge b = Some (External ef) ->
   ef_sig ef = sg ->
-  eval_exprlist pol ge sp e cp m le al vl ->
+  eval_exprlist ge sp e cp m le al vl ->
   transl_exprlist_prop le al vl ->
   external_call ef ge cp vl m E0 v m ->
-  forall (ALLOWED: Policy.allowed_call pol cp (External ef)),
   transl_expr_prop le (Eexternal id sg al) v.
 Proof.
   intros; red; intros. inv TE.
@@ -764,7 +756,6 @@ Proof.
   split. eapply star_trans. eexact EX1.
   eapply star_left. eapply exec_Icall; eauto.
   simpl. rewrite symbols_preserved. rewrite H. eauto. auto.
-  eapply TRANSPOL; eauto. reflexivity.
   eapply star_left. eapply exec_function_external.
   eapply external_call_symbols_preserved; eauto. apply senv_preserved.
   subst cp. eauto.
@@ -795,9 +786,9 @@ Qed.
 Lemma transl_exprlist_Econs_correct:
   forall (le : letenv) (a1 : expr) (al : exprlist) (v1 : val)
          (vl : list val),
-  eval_expr pol ge sp e cp m le a1 v1 ->
+  eval_expr ge sp e cp m le a1 v1 ->
   transl_expr_prop le a1 v1 ->
-  eval_exprlist pol ge sp e cp m le al vl ->
+  eval_exprlist ge sp e cp m le al vl ->
   transl_exprlist_prop le al vl ->
   transl_exprlist_prop le (Econs a1 al) (v1 :: vl).
 Proof.
@@ -823,7 +814,7 @@ Qed.
 
 Lemma transl_condexpr_CEcond_correct:
   forall le cond al vl vb,
-  eval_exprlist pol ge sp e cp m le al vl ->
+  eval_exprlist ge sp e cp m le al vl ->
   transl_exprlist_prop le al vl ->
   eval_condition cond vl m = Some vb ->
   transl_condexpr_prop le (CEcond cond al) vb.
@@ -844,9 +835,9 @@ Qed.
 
 Lemma transl_condexpr_CEcondition_correct:
   forall le a b c va v,
-  eval_condexpr pol ge sp e cp m le a va ->
+  eval_condexpr ge sp e cp m le a va ->
   transl_condexpr_prop le a va ->
-  eval_condexpr pol ge sp e cp m le (if va then b else c) v ->
+  eval_condexpr ge sp e cp m le (if va then b else c) v ->
   transl_condexpr_prop le (if va then b else c) v ->
   transl_condexpr_prop le (CEcondition a b c) v.
 Proof.
@@ -868,9 +859,9 @@ Qed.
 
 Lemma transl_condexpr_CElet_correct:
   forall le a b v1 v2,
-  eval_expr pol ge sp e cp m le a v1 ->
+  eval_expr ge sp e cp m le a v1 ->
   transl_expr_prop le a v1 ->
-  eval_condexpr pol ge sp e cp m (v1 :: le) b v2 ->
+  eval_condexpr ge sp e cp m (v1 :: le) b v2 ->
   transl_condexpr_prop (v1 :: le) b v2 ->
   transl_condexpr_prop le (CElet a b) v2.
 Proof.
@@ -893,9 +884,9 @@ Qed.
 
 Theorem transl_expr_correct:
   forall le a v,
-  eval_expr pol ge sp e cp m le a v ->
+  eval_expr ge sp e cp m le a v ->
   transl_expr_prop le a v.
-Proof (eval_expr_ind3 pol ge sp e cp m
+Proof (eval_expr_ind3 ge sp e cp m
      transl_expr_prop
      transl_exprlist_prop
      transl_condexpr_prop
@@ -915,10 +906,10 @@ Proof (eval_expr_ind3 pol ge sp e cp m
 
 Theorem transl_exprlist_correct:
   forall le a v,
-  eval_exprlist pol ge sp e cp m le a v ->
+  eval_exprlist ge sp e cp m le a v ->
   transl_exprlist_prop le a v.
 Proof
-  (eval_exprlist_ind3 pol ge sp e cp m
+  (eval_exprlist_ind3 ge sp e cp m
      transl_expr_prop
      transl_exprlist_prop
      transl_condexpr_prop
@@ -938,10 +929,10 @@ Proof
 
 Theorem transl_condexpr_correct:
   forall le a v,
-  eval_condexpr pol ge sp e cp m le a v ->
+  eval_condexpr ge sp e cp m le a v ->
   transl_condexpr_prop le a v.
 Proof
-  (eval_condexpr_ind3 pol ge sp e cp m
+  (eval_condexpr_ind3 ge sp e cp m
      transl_expr_prop
      transl_exprlist_prop
      transl_condexpr_prop
@@ -970,14 +961,14 @@ Definition transl_exitexpr_prop
     (ME: match_env map e le rs)
     (EXT: Mem.extends m tm),
   exists nd, exists rs', exists tm',
-     star (step tpol) tge (State cs f sp ns rs tm) E0 (State cs f sp nd rs' tm')
+     star step tge (State cs f sp ns rs tm) E0 (State cs f sp nd rs' tm')
   /\ nth_error nexits x = Some nd
   /\ match_env map e le rs'
   /\ Mem.extends m tm'.
 
 Theorem transl_exitexpr_correct:
   forall le a x,
-  eval_exitexpr pol ge sp e cp m le a x ->
+  eval_exitexpr ge sp e cp m le a x ->
   transl_exitexpr_prop le a x.
 Proof.
   induction 1; red; intros;
@@ -1017,9 +1008,9 @@ Qed.
 
 Lemma eval_exprlist_append:
   forall le al1 vl1 al2 vl2,
-  eval_exprlist pol ge sp e cp m le (exprlist_of_expr_list al1) vl1 ->
-  eval_exprlist pol ge sp e cp m le (exprlist_of_expr_list al2) vl2 ->
-  eval_exprlist pol ge sp e cp m le (exprlist_of_expr_list (al1 ++ al2)) (vl1 ++ vl2).
+  eval_exprlist ge sp e cp m le (exprlist_of_expr_list al1) vl1 ->
+  eval_exprlist ge sp e cp m le (exprlist_of_expr_list al2) vl2 ->
+  eval_exprlist ge sp e cp m le (exprlist_of_expr_list (al1 ++ al2)) (vl1 ++ vl2).
 Proof.
   induction al1; simpl; intros vl1 al2 vl2 E1 E2; inv E1.
 - auto.
@@ -1028,9 +1019,9 @@ Qed.
 
 Lemma invert_eval_builtin_arg:
   forall a v,
-  eval_builtin_arg pol ge sp e cp m a v ->
+  eval_builtin_arg ge sp e cp m a v ->
   exists vl,
-     eval_exprlist pol ge sp e cp m nil (exprlist_of_expr_list (params_of_builtin_arg a)) vl
+     eval_exprlist ge sp e cp m nil (exprlist_of_expr_list (params_of_builtin_arg a)) vl
   /\ Events.eval_builtin_arg ge (fun v => v) sp m (fst (convert_builtin_arg a vl)) v
   /\ (forall vl', convert_builtin_arg a (vl ++ vl') = (fst (convert_builtin_arg a vl), vl')).
 Proof.
@@ -1050,9 +1041,9 @@ Qed.
 
 Lemma invert_eval_builtin_args:
   forall al vl,
-  list_forall2 (eval_builtin_arg pol ge sp e cp m) al vl ->
+  list_forall2 (eval_builtin_arg ge sp e cp m) al vl ->
   exists vl',
-     eval_exprlist pol ge sp e cp m nil (exprlist_of_expr_list (params_of_builtin_args al)) vl'
+     eval_exprlist ge sp e cp m nil (exprlist_of_expr_list (params_of_builtin_args al)) vl'
   /\ Events.eval_builtin_args ge (fun v => v) sp m (convert_builtin_args al vl') vl.
 Proof.
   induction 1; simpl.
@@ -1333,10 +1324,10 @@ Proof.
 Qed.
 
 Theorem transl_step_correct:
-  forall S1 t S2, CminorSel.step pol ge S1 t S2 ->
+  forall S1 t S2, CminorSel.step ge S1 t S2 ->
   forall R1, match_states S1 R1 ->
   exists R2,
-  (plus (RTL.step tpol) tge R1 t R2 \/ (star (RTL.step tpol) tge R1 t R2 /\ lt_state S2 S1))
+  (plus RTL.step tge R1 t R2 \/ (star RTL.step tge R1 t R2 /\ lt_state S2 S1))
   /\ match_states S2 R2.
 Proof.
   induction 1; intros R1 MSTATE; inv MSTATE.
@@ -1406,8 +1397,6 @@ Proof.
   left; eapply plus_right. eapply star_trans. eexact A. eexact E. reflexivity.
   eapply exec_Icall; eauto. simpl. rewrite J. destruct C. eauto. discriminate P. simpl; auto.
   apply sig_transl_function; auto.
-  eapply TRANSPOL; eauto. 
-  rewrite <- COMP; auto.
   traceEq.
   constructor; auto. econstructor; eauto.
   (* direct *)
@@ -1419,8 +1408,6 @@ Proof.
   eapply exec_Icall; eauto. simpl. rewrite symbols_preserved. rewrite H4.
     rewrite Genv.find_funct_find_funct_ptr in P. eauto.
   apply sig_transl_function; auto.
-  eapply TRANSPOL; eauto.
-  rewrite <- COMP; auto.
   traceEq.
   constructor; auto. econstructor; eauto.
 
@@ -1442,8 +1429,6 @@ Proof.
   apply sig_transl_function; auto.
     rewrite <- (comp_transl_partial fd Q), COMP. inv TF; congruence.
   rewrite <- COMP'; eauto.
-  eapply TRANSPOL; eauto.
-  rewrite <- COMP'; auto.
   rewrite H; eauto.
   traceEq.
   constructor; auto.
@@ -1461,8 +1446,6 @@ Proof.
   apply sig_transl_function; auto.
   rewrite <- (comp_transl_partial _ Q), COMP. inv TF; congruence.
   rewrite <- COMP'. eauto.
-  eapply TRANSPOL; eauto.
-  rewrite <- COMP'; auto.
   rewrite H; eauto.
   traceEq.
   constructor; auto.
@@ -1483,7 +1466,6 @@ Proof.
   left. eapply plus_right. eexact E.
   eapply exec_Ibuiltin; eauto.
   eapply eval_builtin_args_preserved with (ge1 := ge); eauto. exact symbols_preserved.
-  rewrite <- COMP; eapply TRANSPOL; eauto. reflexivity.
   eapply external_call_symbols_preserved. apply senv_preserved. eauto.
   rewrite <- COMP. eauto.
   traceEq.
@@ -1642,7 +1624,7 @@ Proof.
 Qed.
 
 Theorem transf_program_correct:
-  forward_simulation (CminorSel.semantics pol prog) (RTL.semantics tpol tprog).
+  forward_simulation (CminorSel.semantics prog) (RTL.semantics tprog).
 Proof.
   eapply forward_simulation_star_wf with (order := lt_state).
   apply senv_preserved.
