backend/Selectionproof.v
@@ -123,7 +123,6 @@ Proof.
   red in H. decompose [Logic.and] H; clear H. red; auto 20.
 Qed.
 
-Definition match_pol (prog: Cminor.program) := Policy.match_pol_gen match_fundef prog.
 
 (** * Correctness of the instruction selection functions for expressions *)
 
@@ -136,8 +135,6 @@ Let tge := Genv.globalenv tprog.
 Hypothesis TRANSF: match_prog prog tprog.
 
 (* Added for interfaces *)
-Variable pol : Cminor.policy.
-Variable tpol : policy.
 Definition match_functions (F : Cminor.function) (F' : function) :=
     Cminor.fn_comp F = F'.(fn_comp)
  /\ Cminor.fn_sig F = F'.(fn_sig).
@@ -145,13 +142,6 @@ Inductive match_fundef_light : (Cminor.fundef) -> fundef -> Prop :=
  | match_fundef_internal : forall f f', match_functions f f' -> match_fundef_light (Internal f) (Internal f')
  | match_fundef_external : forall f, match_fundef_light (External f) (External f).
 
-Hypothesis matching_pol : match_pol prog pol tpol.
-
-Lemma linkorder_policy:
-  forall cunit, linkorder cunit prog ->
-           Policy.match_pol_gen match_fundef prog pol tpol ->
-           Policy.match_pol_gen match_fundef cunit pol tpol.
-Admitted.
 
 Lemma wt_prog : wt_program prog.
 Proof.
@@ -244,9 +234,9 @@ Variable m: mem.
 
 Lemma eval_condexpr_of_expr:
   forall a le v b,
-  eval_expr tpol tge sp e cp m le a v ->
+  eval_expr tge sp e cp m le a v ->
   Val.bool_of_val v b ->
-  eval_condexpr tpol tge sp e cp m le (condexpr_of_expr a) b.
+  eval_condexpr tge sp e cp m le (condexpr_of_expr a) b.
 Proof.
   intros until a. functional induction (condexpr_of_expr a); intros.
 (* compare *)
@@ -263,10 +253,10 @@ Qed.
 
 Lemma eval_condition_of_expr:
   forall a le v b,
-  eval_expr tpol tge sp e cp m le a v ->
+  eval_expr tge sp e cp m le a v ->
   Val.bool_of_val v b ->
   exists vl,
-     eval_exprlist tpol tge sp e cp m le (snd (condition_of_expr a)) vl
+     eval_exprlist tge sp e cp m le (snd (condition_of_expr a)) vl
   /\ eval_condition (fst (condition_of_expr a)) vl m = Some b.
 Proof.
   intros a; functional induction (condition_of_expr a); intros; simpl.
@@ -279,28 +269,28 @@ Qed.
 
 Lemma eval_load:
   forall le a v chunk v',
-  eval_expr tpol tge sp e cp m le a v ->
+  eval_expr tge sp e cp m le a v ->
   Mem.loadv chunk m v = Some v' ->
-  eval_expr tpol tge sp e cp m le (load chunk a) v'.
+  eval_expr tge sp e cp m le (load chunk a) v'.
 Proof.
   intros. generalize H0; destruct v; simpl; intro; try discriminate.
   unfold load.
-  generalize (eval_addressing _ _ _ _ _ _ _ chunk _ _ _ _ H (eq_refl _)).
+  generalize (eval_addressing _ _ _ _ _ _ chunk _ _ _ _ H (eq_refl _)).
   destruct (addressing chunk a). intros [vl [EV EQ]].
   eapply eval_Eload; eauto.
 Qed.
 
 Lemma eval_store:
   forall chunk a1 a2 v1 v2 f k m',
-  eval_expr tpol tge sp e f.(fn_comp) m nil a1 v1 ->
-  eval_expr tpol tge sp e f.(fn_comp) m nil a2 v2 ->
+  eval_expr tge sp e f.(fn_comp) m nil a1 v1 ->
+  eval_expr tge sp e f.(fn_comp) m nil a2 v2 ->
   Mem.storev chunk m v1 v2 = Some m' ->
-  step tpol tge (State f (store chunk a1 a2) k sp e m)
+  step tge (State f (store chunk a1 a2) k sp e m)
         E0 (State f Sskip k sp e m').
 Proof.
   intros. generalize H1; destruct v1; simpl; intro; try discriminate.
   unfold store.
-  generalize (eval_addressing _ _ _ _ _ _ _ chunk _ _ _ _ H (eq_refl _)).
+  generalize (eval_addressing _ _ _ _ _ _ chunk _ _ _ _ H (eq_refl _)).
   destruct (addressing chunk a1). intros [vl [EV EQ]].
   eapply step_store; eauto.
 Qed.
@@ -309,9 +299,9 @@ Qed.
 
 Lemma eval_sel_unop:
   forall le op a1 v1 v,
-  eval_expr tpol tge sp e cp m le a1 v1 ->
+  eval_expr tge sp e cp m le a1 v1 ->
   eval_unop op v1 = Some v ->
-  exists v', eval_expr tpol tge sp e cp m le (sel_unop op a1) v' /\ Val.lessdef v v'.
+  exists v', eval_expr tge sp e cp m le (sel_unop op a1) v' /\ Val.lessdef v v'.
 Proof.
   destruct op; simpl; intros; FuncInv; try subst v.
   apply eval_cast8unsigned; auto.
@@ -351,10 +341,10 @@ Qed.
 
 Lemma eval_sel_binop:
   forall le op a1 a2 v1 v2 v,
-  eval_expr tpol tge sp e cp m le a1 v1 ->
-  eval_expr tpol tge sp e cp m le a2 v2 ->
+  eval_expr tge sp e cp m le a1 v1 ->
+  eval_expr tge sp e cp m le a2 v2 ->
   eval_binop op v1 v2 m = Some v ->
-  exists v', eval_expr tpol tge sp e cp m le (sel_binop op a1 a2) v' /\ Val.lessdef v v'.
+  exists v', eval_expr tge sp e cp m le (sel_binop op a1 a2) v' /\ Val.lessdef v v'.
 Proof.
   destruct op; simpl; intros; FuncInv; try subst v.
   apply eval_add; auto.
@@ -401,11 +391,11 @@ Qed.
 
 Lemma eval_sel_select:
   forall le a1 a2 a3 v1 v2 v3 b ty,
-  eval_expr tpol tge sp e cp m le a1 v1 ->
-  eval_expr tpol tge sp e cp m le a2 v2 ->
-  eval_expr tpol tge sp e cp m le a3 v3 ->
+  eval_expr tge sp e cp m le a1 v1 ->
+  eval_expr tge sp e cp m le a2 v2 ->
+  eval_expr tge sp e cp m le a3 v3 ->
   Val.bool_of_val v1 b ->
-  exists v, eval_expr tpol tge sp e cp m le (sel_select ty a1 a2 a3) v
+  exists v, eval_expr tge sp e cp m le (sel_select ty a1 a2 a3) v
         /\  Val.lessdef (Val.select (Some b) v2 v3 ty) v.
 Proof.
   unfold sel_select; intros.
@@ -423,9 +413,9 @@ Qed.
 Lemma eval_sel_known_builtin:
   forall bf args a vl v le,
   sel_known_builtin bf args = Some a ->
-  eval_exprlist tpol tge sp e cp m le args vl ->
+  eval_exprlist tge sp e cp m le args vl ->
   builtin_function_sem bf vl = Some v ->
-  exists v', eval_expr tpol tge sp e cp m le a v' /\ Val.lessdef v v'.
+  exists v', eval_expr tge sp e cp m le a v' /\ Val.lessdef v v'.
 Proof.
   intros until le; intros SEL ARGS SEM.
   destruct bf as [bf|bf]; simpl in SEL.
@@ -505,17 +495,17 @@ Variable modulus: Z.
 Variable R: Z -> val -> Prop.
 
 Hypothesis eval_make_cmp_eq: forall sp e cp m le a v i n,
-  eval_expr tpol tge sp e cp m le a v -> R i v -> 0 <= n < modulus ->
-  eval_expr tpol tge sp e cp m le (make_cmp_eq a n) (Val.of_bool (zeq i n)).
+  eval_expr tge sp e cp m le a v -> R i v -> 0 <= n < modulus ->
+  eval_expr tge sp e cp m le (make_cmp_eq a n) (Val.of_bool (zeq i n)).
 Hypothesis eval_make_cmp_ltu: forall sp e cp m le a v i n,
-  eval_expr tpol tge sp e cp m le a v -> R i v -> 0 <= n < modulus ->
-  eval_expr tpol tge sp e cp m le (make_cmp_ltu a n) (Val.of_bool (zlt i n)).
+  eval_expr tge sp e cp m le a v -> R i v -> 0 <= n < modulus ->
+  eval_expr tge sp e cp m le (make_cmp_ltu a n) (Val.of_bool (zlt i n)).
 Hypothesis eval_make_sub: forall sp e cp m le a v i n,
-  eval_expr tpol tge sp e cp m le a v -> R i v -> 0 <= n < modulus ->
-  exists v', eval_expr tpol tge sp e cp m le (make_sub a n) v' /\ R ((i - n) mod modulus) v'.
+  eval_expr tge sp e cp m le a v -> R i v -> 0 <= n < modulus ->
+  exists v', eval_expr tge sp e cp m le (make_sub a n) v' /\ R ((i - n) mod modulus) v'.
 Hypothesis eval_make_to_int: forall sp e cp m le a v i,
-  eval_expr tpol tge sp e cp m le a v -> R i v ->
-  exists v', eval_expr tpol tge sp e cp m le (make_to_int a) v' /\ Rint (i mod Int.modulus) v'.
+  eval_expr tge sp e cp m le a v -> R i v ->
+  exists v', eval_expr tge sp e cp m le (make_to_int a) v' /\ Rint (i mod Int.modulus) v'.
 
 Lemma sel_switch_correct_rec:
   forall sp e cp m varg i x,
@@ -524,14 +514,14 @@ Lemma sel_switch_correct_rec:
   wf_comptree modulus t ->
   nth_error le arg = Some varg ->
   comptree_match modulus i t = Some x ->
-  eval_exitexpr tpol tge sp e cp m le (sel_switch make_cmp_eq make_cmp_ltu make_sub make_to_int arg t) x.
+  eval_exitexpr tge sp e cp m le (sel_switch make_cmp_eq make_cmp_ltu make_sub make_to_int arg t) x.
 Proof.
   intros until x; intros Ri. induction t; simpl; intros until le; intros WF ARG MATCH.
 - (* base case *)
   inv MATCH. constructor.
 - (* eq test *)
   inv WF.
-  assert (eval_expr tpol tge sp e cp m le (make_cmp_eq (Eletvar arg) key) (Val.of_bool (zeq i key))).
+  assert (eval_expr tge sp e cp m le (make_cmp_eq (Eletvar arg) key) (Val.of_bool (zeq i key))).
   { eapply eval_make_cmp_eq; eauto. constructor; auto. }
   eapply eval_XEcondition with (va := zeq i key).
   eapply eval_condexpr_of_expr; eauto. destruct (zeq i key); constructor; auto.
@@ -540,7 +530,7 @@ Proof.
   + eapply IHt; eauto.
 - (* lt test *)
   inv WF.
-  assert (eval_expr tpol tge sp e cp m le (make_cmp_ltu (Eletvar arg) key) (Val.of_bool (zlt i key))).
+  assert (eval_expr tge sp e cp m le (make_cmp_ltu (Eletvar arg) key) (Val.of_bool (zlt i key))).
   { eapply eval_make_cmp_ltu; eauto. constructor; auto. }
   eapply eval_XEcondition with (va := zlt i key).
   eapply eval_condexpr_of_expr; eauto. destruct (zlt i key); constructor; auto.
@@ -553,7 +543,7 @@ Proof.
   instantiate (1 := ofs). auto.
   intros (v' & A & B).
   set (i' := (i - ofs) mod modulus) in *.
-  assert (eval_expr tpol tge sp e cp m (v' :: le) (make_cmp_ltu (Eletvar O) sz) (Val.of_bool (zlt i' sz))).
+  assert (eval_expr tge sp e cp m (v' :: le) (make_cmp_ltu (Eletvar O) sz) (Val.of_bool (zlt i' sz))).
   { eapply eval_make_cmp_ltu; eauto. constructor; auto. }
   econstructor. eauto.
   eapply eval_XEcondition with (va := zlt i' sz).
@@ -568,10 +558,10 @@ Qed.
 Lemma sel_switch_correct:
   forall dfl cases arg sp e cp m varg i t le,
   validate_switch modulus dfl cases t = true ->
-  eval_expr tpol tge sp e cp m le arg varg ->
+  eval_expr tge sp e cp m le arg varg ->
   R i varg ->
   0 <= i < modulus ->
-  eval_exitexpr tpol tge sp e cp m le
+  eval_exitexpr tge sp e cp m le
      (XElet arg (sel_switch make_cmp_eq make_cmp_ltu make_sub make_to_int O t))
      (switch_target i dfl cases).
 Proof.
@@ -595,11 +585,11 @@ Qed.
 Lemma sel_switch_int_correct:
   forall dfl cases arg sp e cp m i t le,
   validate_switch Int.modulus dfl cases t = true ->
-  eval_expr tpol tge sp e cp m le arg (Vint i) ->
-  eval_exitexpr tpol tge sp e cp m le (XElet arg (sel_switch_int O t)) (switch_target (Int.unsigned i) dfl cases).
+  eval_expr tge sp e cp m le arg (Vint i) ->
+  eval_exitexpr tge sp e cp m le (XElet arg (sel_switch_int O t)) (switch_target (Int.unsigned i) dfl cases).
 Proof.
   assert (INTCONST: forall n sp e cp m le,
-            eval_expr tpol tge sp e cp m le (Eop (Ointconst n) Enil) (Vint n)).
+            eval_expr tge sp e cp m le (Eop (Ointconst n) Enil) (Vint n)).
   { intros. econstructor. constructor. auto. }
   intros. eapply sel_switch_correct with (R := Rint); eauto.
 - intros until n; intros EVAL R RANGE.
@@ -635,8 +625,8 @@ Qed.
 Lemma sel_switch_long_correct:
   forall dfl cases arg sp e cp m i t le,
   validate_switch Int64.modulus dfl cases t = true ->
-  eval_expr tpol tge sp e cp m le arg (Vlong i) ->
-  eval_exitexpr tpol tge sp e cp m le (XElet arg (sel_switch_long O t)) (switch_target (Int64.unsigned i) dfl cases).
+  eval_expr tge sp e cp m le arg (Vlong i) ->
+  eval_exitexpr tge sp e cp m le (XElet arg (sel_switch_long O t)) (switch_target (Int64.unsigned i) dfl cases).
 Proof.
   intros. eapply sel_switch_correct with (R := Rlong); eauto.
 - intros until n; intros EVAL R RANGE.
@@ -774,7 +764,7 @@ Lemma sel_expr_correct:
   Cminor.eval_expr ge sp e m a v ->
   forall e' le m',
   env_lessdef e e' -> Mem.extends m m' ->
-  exists v', eval_expr tpol tge sp e' cp m' le (sel_expr a) v' /\ Val.lessdef v v'.
+  exists v', eval_expr tge sp e' cp m' le (sel_expr a) v' /\ Val.lessdef v v'.
 Proof.
   induction 1; intros; simpl.
   (* Evar *)
@@ -796,7 +786,7 @@ Proof.
   exploit IHeval_expr1; eauto. intros [v1' [A B]].
   exploit IHeval_expr2; eauto. intros [v2' [C D]].
   exploit eval_binop_lessdef; eauto. intros [v' [E F]].
-  assert (G: exists v'', eval_expr tpol tge sp e' cp m' le (sel_binop op (sel_expr a1) (sel_expr a2)) v'' /\ Val.lessdef v' v'')
+  assert (G: exists v'', eval_expr tge sp e' cp m' le (sel_binop op (sel_expr a1) (sel_expr a2)) v'' /\ Val.lessdef v' v'')
   by (eapply eval_sel_binop; eauto).
   destruct G as [v'' [P Q]].
   exists v''; split; eauto. eapply Val.lessdef_trans; eauto.
@@ -811,7 +801,7 @@ Lemma sel_exprlist_correct:
   Cminor.eval_exprlist ge sp e m a v ->
   forall e' le m',
   env_lessdef e e' -> Mem.extends m m' ->
-  exists v', eval_exprlist tpol tge sp e' cp m' le (sel_exprlist a) v' /\ Val.lessdef_list v v'.
+  exists v', eval_exprlist tge sp e' cp m' le (sel_exprlist a) v' /\ Val.lessdef_list v v'.
 Proof.
   induction 1; intros; simpl.
   exists (@nil val); split; auto. constructor.
@@ -828,7 +818,7 @@ Lemma sel_select_opt_correct:
   Cminor.eval_expr ge sp e m a2 v2 ->
   Val.bool_of_val vcond b ->
   env_lessdef e e' -> Mem.extends m m' ->
-  exists v', eval_expr tpol tge sp e' cp m' le a v' /\ Val.lessdef (Val.select (Some b) v1 v2 ty) v'.
+  exists v', eval_expr tge sp e' cp m' le a v' /\ Val.lessdef (Val.select (Some b) v1 v2 ty) v'.
 Proof.
   unfold sel_select_opt; intros. 
   destruct (condition_of_expr (sel_expr cond)) as [cnd args] eqn:C.
@@ -848,7 +838,7 @@ Lemma sel_builtin_arg_correct:
   env_lessdef e e' -> Mem.extends m m' ->
   Cminor.eval_expr ge sp e m a v ->
   exists v',
-     CminorSel.eval_builtin_arg tpol tge sp e' cp m' (sel_builtin_arg a c) v'
+     CminorSel.eval_builtin_arg tge sp e' cp m' (sel_builtin_arg a c) v'
   /\ Val.lessdef v v'.
 Proof.
   intros. unfold sel_builtin_arg.
@@ -866,7 +856,7 @@ Lemma sel_builtin_args_correct:
   Cminor.eval_exprlist ge sp e m al vl ->
   forall cl,
   exists vl',
-     list_forall2 (CminorSel.eval_builtin_arg tpol tge sp e' cp m')
+     list_forall2 (CminorSel.eval_builtin_arg tge sp e' cp m')
                   (sel_builtin_args al cl)
                   vl'
   /\ Val.lessdef_list vl vl'.
@@ -891,9 +881,9 @@ Lemma sel_builtin_default_correct:
   Cminor.eval_exprlist ge sp e1 m1 al vl ->
   external_call ef ge f.(fn_comp) vl m1 t v m2 ->
   env_lessdef e1 e1' -> Mem.extends m1 m1' ->
-  forall ALLOWED: Policy.allowed_call tpol f.(fn_comp) (External ef),
+  (* forall ALLOWED: Policy.allowed_call f.(fn_comp) (External ef), *)
   exists e2' m2',
-     step tpol tge (State f (sel_builtin_default optid ef al) k sp e1' m1')
+     step tge (State f (sel_builtin_default optid ef al) k sp e1' m1')
             t (State f Sskip k sp e2' m2')
   /\ env_lessdef (set_optvar optid v e1) e2'
   /\ Mem.extends m2 m2'.
@@ -913,9 +903,9 @@ Lemma sel_builtin_correct:
   Cminor.eval_exprlist ge sp e1 m1 al vl ->
   external_call ef ge f.(fn_comp) vl m1 t v m2 ->
   env_lessdef e1 e1' -> Mem.extends m1 m1' ->
-  forall ALLOWED: Policy.allowed_call tpol f.(fn_comp) (External ef),
+  (* forall ALLOWED: Policy.allowed_call f.(fn_comp) (External ef), *)
   exists e2' m2',
-     step tpol tge (State f (sel_builtin optid ef al) k sp e1' m1')
+     step tge (State f (sel_builtin optid ef al) k sp e1' m1')
             t (State f Sskip k sp e2' m2')
   /\ env_lessdef (set_optvar optid v e1) e2'
   /\ Mem.extends m2 m2'.
@@ -940,7 +930,7 @@ Qed.
 Lemma classify_stmt_sound_1:
   forall f sp e m s k,
   classify_stmt s = SCskip ->
-  star (Cminor.step pol) ge (Cminor.State f s k sp e m) E0 (Cminor.State f Cminor.Sskip k sp e m).
+  star Cminor.step ge (Cminor.State f s k sp e m) E0 (Cminor.State f Cminor.Sskip k sp e m).
 Proof.
   intros until s; functional induction (classify_stmt s); intros; try discriminate.
   - apply star_refl.
@@ -956,7 +946,7 @@ Lemma classify_stmt_sound_2:
   Cminor.eval_expr ge sp e m a v ->
   forall s k,
   classify_stmt s = SCassign id a ->
-  star (Cminor.step pol) ge (Cminor.State f s k sp e m) E0 (Cminor.State f Cminor.Sskip k sp (PTree.set id v e) m).
+  star Cminor.step ge (Cminor.State f s k sp e m) E0 (Cminor.State f Cminor.Sskip k sp (PTree.set id v e) m).
 Proof.
   intros until s; functional induction (classify_stmt s); intros; try discriminate.
   - inv H0. apply star_one. constructor; auto.
@@ -995,7 +985,7 @@ Lemma eval_select_safe_exprs:
      s = Sassign id a'
   /\ Cminor.eval_expr ge sp e m a1 v1
   /\ Cminor.eval_expr ge sp e m a2 v2
-  /\ eval_expr tpol tge sp e' cp m' nil a' v'
+  /\ eval_expr tge sp e' cp m' nil a' v'
   /\ Val.lessdef (if b then v1 else v2) v'.
 Proof.
   intros.
@@ -1021,8 +1011,8 @@ Lemma if_conversion_correct:
   env_lessdef e e' -> Mem.extends m m' ->
   let s0 := if b then ifso else ifnot in
   exists e1 e1',
-     step tpol tge (State f' s k' sp e' m') E0 (State f' Sskip k' sp e1' m')
-  /\ star (Cminor.step pol) ge (Cminor.State f s0 k sp e m) E0 (Cminor.State f Cminor.Sskip k sp e1 m)
+     step tge (State f' s k' sp e' m') E0 (State f' Sskip k' sp e1' m')
+  /\ star Cminor.step ge (Cminor.State f s0 k sp e m) E0 (Cminor.State f Cminor.Sskip k sp e1 m)
   /\ env_lessdef e1 e1'.
 Proof.
   unfold if_conversion; intros until m'; intros IFC DE WTE WT1 WT2 EVC BOV ELD MEXT.
@@ -1298,11 +1288,11 @@ Definition measure (s: Cminor.state) : nat :=
   end.
 
 Lemma sel_step_correct:
-  forall S1 t S2, Cminor.step pol ge S1 t S2 ->
+  forall S1 t S2, Cminor.step ge S1 t S2 ->
   forall T1, match_states S1 T1 -> wt_state S1 ->
-  (exists T2, step tpol tge T1 t T2 /\ match_states S2 T2)
+  (exists T2, step tge T1 t T2 /\ match_states S2 T2)
   \/ (measure S2 < measure S1 /\ t = E0 /\ match_states S2 T1)%nat
-  \/ (exists S3 T2, star (Cminor.step pol) ge S2 E0 S3 /\ step tpol tge T1 t T2 /\ match_states S3 T2).
+  \/ (exists S3 T2, star Cminor.step ge S2 E0 S3 /\ step tge T1 t T2 /\ match_states S3 T2).
 Proof.
   induction 1; intros T1 ME WTS; inv ME; try (monadInv TS).
 - (* skip seq *)
@@ -1339,8 +1329,7 @@ Proof.
   left; econstructor; split.
   econstructor; eauto. econstructor; eauto.
   eapply sig_function_translated; eauto.
-  eapply linkorder_policy with (cunit := cunit'); eauto.
-  rewrite CPT in ALLOWED; eauto.
+  rewrite CPT in ALLOWED; eauto. admit.
   eapply match_callstate with (cunit := cunit'); eauto.
   eapply match_cont_call with (cunit := cunit) (hf := hf); eauto.
 + (* direct *)
@@ -1351,8 +1340,7 @@ Proof.
   econstructor; eauto.
   subst vf. econstructor; eauto. rewrite symbols_preserved; eauto.
   eapply sig_function_translated; eauto.
-  eapply linkorder_policy with (cunit := cunit'); eauto.
-  rewrite CPT in ALLOWED; eauto.
+  rewrite CPT in ALLOWED; eauto. admit.
   eapply match_callstate with (cunit := cunit'); eauto.
   eapply match_cont_call with (cunit := cunit) (hf := hf); eauto.
 + (* turned into Sbuiltin *)
@@ -1370,25 +1358,20 @@ Proof.
   econstructor; eauto. econstructor; eauto. eapply sig_function_translated; eauto.
   rewrite <- (comp_function_translated _ _ _ F), COMP. now apply (comp_transl_partial _ TF).
   rewrite <- CPT; trivial.
-  eapply linkorder_policy with (cunit := cunit'); eauto.
-  rewrite CPT in ALLOWED'; eauto.
+  rewrite CPT in ALLOWED'; eauto. admit.
   destruct H2 as [b [U V]]. subst vf. inv B.
   econstructor; eauto. econstructor; eauto. rewrite symbols_preserved; eauto. eapply sig_function_translated; eauto.
   rewrite <- (comp_function_translated _ _ _ F), COMP. now apply (comp_transl_partial _ TF).
   rewrite <- CPT; trivial.
-  eapply linkorder_policy with (cunit := cunit'); eauto.
-  rewrite CPT in ALLOWED'; eauto.
+  rewrite CPT in ALLOWED'; eauto. admit.
   econstructor; eauto. econstructor; eauto. eapply sig_function_translated; eauto.
   rewrite <- (comp_function_translated _ _ _ F), COMP. now apply (comp_transl_partial _ TF).
   rewrite <- CPT; trivial.
-  eapply linkorder_policy with (cunit := cunit'); eauto.
-  rewrite CPT in ALLOWED'; eauto.
+  rewrite CPT in ALLOWED'; eauto. admit.
   eapply match_callstate with (cunit := cunit'); eauto.
   eapply call_cont_commut; eauto.
 - (* Sbuiltin *)
   exploit sel_builtin_correct; eauto; try (now erewrite <- CPT; eauto).
-  eapply linkorder_policy with (cunit := cunit) (f := External ef); eauto.
-  econstructor; split; eauto. rewrite <- CPT; eauto.
   intros (e2' & m2' & P & Q & R).
   left; econstructor; split. eexact P. econstructor; eauto.
 - (* Seq *)
@@ -1483,9 +1466,6 @@ Proof.
   econstructor; eauto.
 - (* external call turned into a Sbuiltin *)
   exploit sel_builtin_correct; eauto. rewrite <- CPT; eauto.
-  eapply linkorder_policy with (cunit := cunit) (f := External ef); eauto.
-  econstructor; split; eauto. rewrite <- CPT; eauto.
-  admit.
   intros (e2' & m2' & P & Q & R).
   left; econstructor; split. eexact P. econstructor; eauto.
 - (* return *)
@@ -1520,7 +1500,7 @@ Proof.
 Qed.
 
 Theorem transf_program_correct:
-  forward_simulation (Cminor.semantics pol prog) (CminorSel.semantics tpol tprog).
+  forward_simulation (Cminor.semantics prog) (CminorSel.semantics tprog).
 Proof.
   set (MS := fun S T => match_states S T /\ wt_state S).
   apply forward_simulation_determ_star with (match_states := MS) (measure := measure).
